Runtime/Network/Graph/Path/Sibling.lean
@@ -1,0 +1,38 @@
+import Runtime.Network.Graph.Path.Extends
+
+namespace Network.Graph.Path
+
+-- Note: Every node except for the start can be its own sibling.
+def Sibling (path₁ path₂ : Path graph start) :=
+  ∃ parent, (path₁ ≻ parent) ∧ (path₂ ≻ parent)
+
+infix:35 " ≂ " => Sibling
+
+theorem Sibling.symm : (path₁ ≂ path₂) → (path₂ ≂ path₁) := 
+  fun ⟨parent, h₁, h₂⟩ => ⟨parent, h₂, h₁⟩
+
+theorem Sibling.isCons₁ : (path₁ ≂ path₂) → path₁.isCons :=
+  fun ⟨_, h, _⟩ => h.isCons
+
+theorem Sibling.isCons₂ : (path₁ ≂ path₂) → path₂.isCons := 
+  fun ⟨_, _, h⟩ => h.isCons
+
+theorem Sibling.to_eq_prefix : (path₁ ≂ path₂) → (path₁.prefix = path₂.prefix) := by
+  intro ⟨_, _, _⟩
+  simp_all [Extends.iff_prefix]
+
+theorem Sibling.of_eq_prefix : (path₁.prefix = some parent) → (path₂.prefix = some parent) → (path₁ ≂ path₂) := by
+  intro h₁ h₂
+  simp [←Extends.iff_prefix] at h₁ h₂
+  exact ⟨_, h₁, h₂⟩
+
+instance : Decidable (path₁ ≂ path₂) :=
+  match h₁ : path₁.prefix, h₂ : path₂.prefix with
+  | none, _ => .isFalse (by have := isCons_prefix_isSome ·.isCons₁; simp_all [Option.isSome])
+  | _, none => .isFalse (by have := isCons_prefix_isSome ·.isCons₂; simp_all [Option.isSome])
+  | some pre₁, some pre₂ =>
+    if h : pre₁ = pre₂ 
+    then .isTrue (Sibling.of_eq_prefix h₁ (h ▸ h₂))
+    else .isFalse (by simp_all [mt Sibling.to_eq_prefix])
+
+end Network.Graph.Path
